relations: refactoring

relations.v
@@ -1,5 +1,5 @@
 From Coq Require Import Lia.
-From Coq Require Import Relations Program.Basics.
+From Coq Require Import Relations Program.Basics ssrsearch.
 From mathcomp Require Import ssreflect ssrbool eqtype ssrfun seq order.
 From Equations Require Import Equations.
 From event_struct Require Import utilities wftype.
@@ -13,133 +13,153 @@ Open Scope order_scope.
 
 Section well_founded.
 
+Definition sfrel {T : eqType} (f : T -> seq T) : rel T :=
+  [rel a b | b \in f a].
+
+Definition filter_neq {T : eqType} (f : T -> seq T) : T -> seq T :=
+  fun n => filter^~ (f n) (fun x => x != n).
+
+Notation "f '\eq'" := (filter_neq f) (at level 5, format "f '\eq'").
+
 Context {T : wfType}.
-
-Definition filter_neq (f : T -> seq T) : T -> seq T :=
-  fun n => filter (fun x => x != n) (f n).
-
-Definition sfrel (f : T -> seq T) : rel T :=
-  [rel a b | a \in (filter_neq f) b].
 
 Variable (f : T -> seq T).
 
 Hypothesis descend : forall x n, x \in f n -> x <= n.
 
-Lemma filter_lt n k : k \in (filter_neq f n) -> k < n.
+Lemma filter_lt n k : k \in f\eq n -> k < n.
 Proof. by rewrite mem_filter lt_neqAle => /andP[] -> /descend ->. Qed.
 
-Lemma rel_sublt a b : (sfrel f) a b -> a < b.
+Lemma rel_sublt a b : (sfrel f\eq) a b -> b < a.
 Proof. rewrite/sfrel /=. exact: filter_lt. Qed.
 
-(* Well-founded relation closure definition *)
-Equations(noind) t_closure (n : T) : seq T by wf n (<%O : rel T) :=
-  t_closure n := 
-    let ys := (filter_neq f n) in 
+(* Computation of the strict upward set of a given element
+ * w.r.t relation R derived from function `f`,
+ * i.e. s_up_set(x) = { y | x R y } 
+ *)
+Equations(noind) s_up_set (n : T) : seq T by wf n (<%O : rel T) :=
+  s_up_set n := 
+    let ys := f\eq n in 
     let ps := flatten (map^~ ys (fun x => 
       if x \in ys =P true is ReflectT pf then
-        t_closure x
+        s_up_set x
       else 
         [::]
     )) in
     ys ++ ps.
 Next Obligation. exact: filter_lt. Qed.
 
-Definition rel_of_closure (a b : T) : bool := a \in t_closure b.
+Definition t_closure (a b : T) : bool := b \in s_up_set a.
 
-Lemma ext_t_closure (x : T) (g h : forall y : T, y < x -> seq T) :
+Lemma ext_s_up_set (x : T) (g h : forall y : T, y < x -> seq T) :
   (forall (y : T) (p : y < x), g y p = h y p) ->
-    t_closure_functional x g = t_closure_functional x h.
+    s_up_set_functional x g = s_up_set_functional x h.
 Proof.
-  move=> H. rewrite /t_closure_functional. apply/eqP.
+  move=> H. rewrite /s_up_set_functional. apply/eqP.
   rewrite eqseq_cat //=. apply/andP. split=> //=. apply/eqP.
   congr flatten. apply/eq_in_map. move=> y /filter_lt. case: eqP=> //=.
 Qed.
 
-Lemma rel_of_closure_sublt a b : rel_of_closure a b -> a < b.
+Lemma t_closure_lt a b : t_closure a b -> b < a.
 Proof.
-  rewrite /rel_of_closure.
-  move: b a. apply: wf_ind => b IH a.
-  rewrite /t_closure /Subterm.FixWf Fix_eq; last by apply: ext_t_closure.
-  rewrite {1}/t_closure_functional mem_cat => /orP [/filter_lt //|].
+  rewrite /t_closure.
+  move: a b. apply: wf_ind => a IH b.
+  rewrite /s_up_set /Subterm.FixWf Fix_eq; last by apply: ext_s_up_set.
+  rewrite {1}/s_up_set_functional mem_cat => /orP [/filter_lt //|].
   case/flatten_mapP=> x /filter_lt xinf.
   case: eqP => //. move=> /filter_lt /IH /apply ax. 
   by apply: lt_trans; first apply: ax.
 Qed.
 
-Lemma clos_trans_sublt a b : clos_trans_n1 T (sfrel f) a b -> a < b.
+Lemma clos_trans_lt a b : clos_trans_n1 T (sfrel f\eq) a b -> b < a.
 Proof.
   rewrite/sfrel /=.
   elim=> [x /filter_lt // | x y xfy acx ax].
-  apply: lt_trans; first by apply: ax.
+  apply: lt_trans; last by apply: ax.
   exact: filter_lt.
 Qed. 
 
-(* Well-founded relations properties *)
-Lemma closureP a b : 
-  reflect (clos_trans_n1 T (sfrel f) a b) (rel_of_closure a b).
+(* Transitive closure reflection lemma *)
+Lemma t_closureP a b : 
+  reflect (clos_trans_1n T (sfrel f\eq) a b) (t_closure a b).
 Proof.
-  rewrite /rel_of_closure.
-  move: b a. apply: wf_ind=> b IH a.
+  rewrite /t_closure.
+  move: a b. apply: wf_ind=> a IH b.
   apply /(iffP idP).
-  { rewrite /t_closure /Subterm.FixWf Fix_eq; last by apply: ext_t_closure.
-    rewrite {1}/t_closure_functional mem_cat => /orP [].
+  { rewrite /s_up_set /Subterm.FixWf Fix_eq; last by apply: ext_s_up_set.
+    rewrite {1}/s_up_set_functional mem_cat => /orP [].
     { by constructor. }
     case/flatten_mapP=> x xinf. case: eqP=> //=.
-    move=> /filter_lt /IH /apply H. 
-    apply /clos_trans_tn1 /t_trans; first last.
-    { constructor. apply: xinf. }
-    apply /clos_tn1_trans. exact: H. }
+    move=> /filter_lt /IH /apply H.
+    apply: Relation_Operators.t1n_trans; last exact H.
+    exact xinf. }
   move=> ctab. move: ctab IH. case.
   { rewrite /sfrel /= => c afc IH.
-    rewrite /t_closure /Subterm.FixWf Fix_eq; last by apply: ext_t_closure.
-    by rewrite {1}/t_closure_functional mem_cat afc. }
+    rewrite /s_up_set /Subterm.FixWf Fix_eq; last by apply: ext_s_up_set.
+    by rewrite {1}/s_up_set_functional mem_cat afc. }
   move=> c d. rewrite /sfrel /= => cfd ctac IHd.
-  rewrite /t_closure /Subterm.FixWf Fix_eq; last by apply: ext_t_closure.
-  rewrite {1}/t_closure_functional mem_cat. apply/orP.
+  rewrite /s_up_set /Subterm.FixWf Fix_eq; last by apply: ext_s_up_set.
+  rewrite {1}/s_up_set_functional mem_cat. apply/orP.
   right. apply/flatten_mapP. exists c=> //=. case: eqP=> //=.
   move=> _. apply/IHd=> //=. exact: filter_lt.
 Qed.
 
-(* reflexive-transitive closure definition *)
-Definition rt_closure a := a :: t_closure a.
 
-Definition rt_closure_rel a b := a \in rt_closure b. 
+(* Computation of the (non-strict) upward set of a given element
+ * w.r.t relation R derived from function `f`,
+ * i.e. up_set(x) = { y | x = y \/ x R y } 
+ *)
+Definition up_set a := a :: s_up_set a.
 
-Lemma rt_closure_refl a : rt_closure_rel a a.
-Proof.
-  rewrite /rt_closure_rel /rt_closure. exact: mem_head.
-Qed.
+Definition rt_closure a b := b \in up_set a. 
+
+Lemma rt_closure_refl a : rt_closure a a.
+Proof. rewrite /rt_closure /up_set. exact: mem_head. Qed.
 
 Lemma rt_closure_trans a b c :
-  rt_closure_rel a b -> rt_closure_rel b c -> rt_closure_rel a c.
+  rt_closure a b -> rt_closure b c -> rt_closure a c.
 Proof.
-  rewrite /rt_closure_rel.
-  rewrite !in_cons => /orP[/eqP -> //| atb /orP [ /eqP <-| btc]]; first by rewrite atb.
-  apply/orP. right. apply/closureP. apply: clos_trans_tn1. apply: t_trans.
-  { apply /clos_tn1_trans /closureP. exact: atb. }
-  apply /clos_tn1_trans /closureP. exact: btc.
+  rewrite /rt_closure.
+  rewrite !in_cons => /orP [/eqP -> //|].
+  move=> ba /orP [/eqP -> //|].
+  { by rewrite ba. }
+  move=> cb. apply /orP. right.
+  apply /t_closureP. apply: clos_trans_t1n. apply: t_trans.
+  { apply /clos_t1n_trans /t_closureP. exact: ba. }
+  apply /clos_t1n_trans /t_closureP. exact: cb.
 Qed.
 
+(* Reflexive-transitive closure reflection lemma *)
 Lemma rt_closureP a b :
-  reflect (clos_refl_trans_n1 T (sfrel f) a b) (rt_closure_rel a b).
+  reflect (clos_refl_trans_1n T (sfrel f) a b) (rt_closure a b).
 Proof.
   apply /(iffP idP).
-  { rewrite /rt_closure_rel. rewrite in_cons=> /orP[/eqP -> | atb].
+  { rewrite /rt_closure. 
+    rewrite in_cons=> /orP[/eqP -> | atb].
     { constructor. }
-    move: (closureP a b). rewrite/rel_of_closure => refl.
-    move: (refl atb). elim=> [c afc | c d cfd cac crac].
-    { apply: rtn1_trans; first by apply: afc. constructor. }
-    apply: rtn1_trans; first by apply: cfd. done. }
-  move=> cab. rewrite /rt_closure_rel /rt_closure.
+    move: (t_closureP a b). 
+    rewrite /t_closure => refl. move: (refl atb). 
+    elim=> [c d cfd | c d e cfd st rt].
+    { apply: Relation_Operators.rt1n_trans; last by constructor.
+      move: cfd. rewrite /sfrel /filter_neq //=.
+      rewrite mem_filter. by move=> /andP [??]. }
+    apply: Relation_Operators.rt1n_trans; last exact: rt.
+    move: cfd. rewrite /sfrel /filter_neq //=.
+    rewrite mem_filter. move=> /andP [? H]. exact: H. }
+  move=> cab. rewrite /rt_closure /up_set.
   rewrite in_cons. apply/orP.
-  elim: cab => [| c d cfd crac [/eqP -> | ac]]; first by left.
-  { right. move: cfd. rewrite /sfrel /=.
-    rewrite /t_closure /Subterm.FixWf Fix_eq; last by apply: ext_t_closure.
-    by rewrite {1}/t_closure_functional mem_cat => ->. }
-  right. move: (closureP a c)=> refl. move: (refl ac)=> cac.
-  apply /(closureP a d) /clos_trans_tn1 /t_trans.
-  { apply /clos_tn1_trans. exact: cac. }
-  by constructor.
+  elim: cab => [| c d e st rt [/eqP -> | efd]]; first by left.
+  { case: (d =P c)=> [eq|neq] //=; first by left.
+    right. move: st. rewrite /sfrel /=.
+    rewrite /s_up_set /Subterm.FixWf Fix_eq; last by apply: ext_s_up_set.
+    rewrite {1}/s_up_set_functional mem_cat /filter_neq mem_filter => ->.
+     apply /orP. left. by apply /predD1P. }
+  case: (d =P c)=> [<-|neq] //=; first by right. 
+  right. move: (t_closureP d e)=> refl. move: (refl efd)=> ct.
+  apply /(t_closureP c e) /clos_trans_t1n /t_trans; first last.
+  { apply: clos_t1n_trans. exact: ct. }
+  apply: t_step. rewrite /sfrel /filter_neq //=. 
+  rewrite mem_filter. by apply /predD1P. 
 Qed.
 
 End well_founded.
